Ready/Unready states

disk-betree/BlockCache.dfy
@@ -1,15 +1,16 @@
-
+include "DiskBetree.dfy"
 
 module BlockCache {
   datatype Constants = Constants()
 
   // psssst T = Node but dodn't tell anybody
-  type T = Node
+  import DiskBetree
+  type T<Value> = DiskBetree.Node<Value>
   function Successor(node: T): iset<Reference> { node.children.Values }
 
   // Stuff for communicating with Disk (probably move to another file?)
 
-  type Superblock = map<Reference, LBA>
+  type Superblock = map<Reference, (LBA, refcount)>
 
   datatype Sector =
     | SectorBlock(block: T)
@@ -26,27 +27,33 @@ module BlockCache {
   datatype Status = Dirty | Clean
   datatype CacheLine<T> = CacheLine(block: T, status: Status)
 
-  datatype Variables = Variables(
-      persistentSuperblock: SuperBlock,
-      ephemeralSuperblock: SuperBlock,
-      cache: map<Reference, CacheLine>);
+  datatype Variables =
+    | Ready(
+        persistentSuperblock: SuperBlock?,
+        ephemeralSuperblock: SuperBlock?,
+        cache: map<Reference, CacheLine>)
+    | Unready(
+        cache: map<Reference, CacheLine>)
 
   datatype Step =
     | WriteBackStep(ref: Reference)
     | WriteBackSuperblockStep
     | DirtyStep(ref: Reference, block: T)
-    | PageInStep
+    | Unalloc(ref: Reference)
+    | PageInStep(ref: Reference)
+    | PageInSuperblockStep
     | EvictStep(ref: Reference)
-    // TODO unalloc
     // TODO page in superblock
 
   predicate WriteBack(k: Constants, s: Variables, s': Variables, dop: DiskOp, ref: Reference)
   {
+    && s.Ready?
     && dop.Write?
     && ref in s.cache
     && dop.lba !in persistentSuperblock.Values
     && dop.lba !in ephemeralSuperblock.Values
     && dop.sector == SectorBlock(s.cache[dop.lba].block)
+    && s'.Ready?
     && s'.persistentSuperblock == s.persistentSuperblock
     && s'.ephemeralSuperblock == s.ephemeralSuperblock[ref := dop.lba]
     && s'.cache == s.cache[ref := s.cache[ref][status := Clean]]
@@ -54,6 +61,7 @@ module BlockCache {
 
   predicate WriteBackSuperblock(k: Constants, s: Variables, s': Variables, dop: DiskOp)
   {
+    && s.Ready?
     && dop.Write?
     && dop.lba == SuperblockLBA(k)
     && dop.sector == SectorSuperblock(s.ephemeralSuperblock)
@@ -68,8 +76,20 @@ module BlockCache {
     && s' == s[cache := s.cache[ref := CacheLine(block, Dirty)]]
   }
 
+  predicate Unalloc(k: Constants, s: Variables, s': Variables, dop: DiskOp, ref: Reference)
+  {
+    && s.Ready?
+    && dop.NoDiskOp
+    && ref in s.ephemeralSuperblock
+    && s'.Ready?
+    && s'.persistentSuperblock == s.persistentSuperblock
+    && s'.ephemeralSuperblock == RemoveFromMap(s.ephemeralSuperblock, ref)
+    && s'.cache == RemoveFromMap(s.cache, ref)
+  }
+
   predicate PageIn(k: Constants, s: Variables, s': Variables, dop: DiskOp, ref: Reference)
   {
+    && s.Ready?
     && dop.Read
     && ref in s.cache ==> s.cache[ref].status == Clean
     && ref in s.ephemeralSuperblock
@@ -78,8 +98,18 @@ module BlockCache {
     && s' == s[cache := s.cache[ref := CacheLine(dop.sector.block, Clean)]]
   }
 
+  predicate PageInSuperblock(k: Constants, s: Variables, s': Variables, dop: DiskOp, ref: Reference)
+  {
+    && s.Unready?
+    && dop.Read
+    && dop.lba == SuperblockLBA
+    && dop.sector.superblock?
+    && s' == Ready(dop.sector.superblock, dop.sector.superblock, s.cache)
+  }
+
   predicate Evict(k: Constants, s: Variables, s': Variables, dop: DiskOp, ref: Reference)
   {
+    && s.Ready?
     && dop.NoDiskOp
     && ref in s.cache
     && s.cache[ref].status == Clean
@@ -91,10 +121,22 @@ module BlockCache {
     SuperBlockLBA !in superblock.Values
   }
 
+  predicate Init(k: Constants, s: Variables)
+  {
+    s == Unready(map[])
+  }
+
   predicate Inv(k: Constants, s: Variables)
   {
-    && WFSuperblock(s.persistentSuperblock)
-    && WFSuperblock(s.ephemeralSuperblock)
-    && (forall ref in s.cache.keys :: s.cache.keys[ref].status == Clean ==> ref in s.ephemeralSuperblock)
+    match s {
+      case Ready(persistentSuperblock, ephemeralSuperblock, cache) => {
+        && WFSuperblock(s.persistentSuperblock)
+        && WFSuperblock(s.ephemeralSuperblock)
+        && (forall ref :: ref in s.cache.keys && s.cache.keys[ref].status == Clean ==> ref in s.ephemeralSuperblock)
+      }
+      case Unready(cache) => {
+        && (forall ref :: ref in s.cache.keys && s.cache.keys[ref].status == Dirty)
+      }
+    }
   }
 }
